michael_formal/examples/Drinks_Machine.thy
@@ -111,7 +111,7 @@ lemma possible_steps_q0:  "length i = Suc 0 \<Longrightarrow> possible_steps dri
       apply (meson empty_iff old.prod.inject singletonD statename.distinct(1))
   by (simp_all add: select_def)
 
-lemma select_updates [simp]: "(EFSM.apply_updates (Updates select) (case_vname (\<lambda>n. if n = Suc 0 then Some (Str ''coke'') else index2state [] (Suc 0 + 1) (I n)) Map.empty) Map.empty) = <R 1:=Str ''coke'', R 2 := Num 0>"
+lemma select_updates [simp]: "(EFSM.apply_updates (Updates select) (case_vname (\<lambda>n. if n = Suc 0 then Some (Str ''coke'') else input2state [] (Suc 0 + 1) (I n)) Map.empty) Map.empty) = <R 1:=Str ''coke'', R 2 := Num 0>"
   apply (simp add: select_def)
   apply (rule ext)
   by simp
@@ -162,7 +162,7 @@ lemma possible_steps_q1_coin_2: "possible_steps drinks q1 <R (Suc 0) := Str ''co
   by (simp_all add: drinks_def coin_def)
 
 lemma coin_updates [simp]: "(EFSM.apply_updates (Updates coin)
-               (case_vname (\<lambda>n. if n = Suc 0 then Some (Num i) else index2state [] (Suc 0 + 1) (I n)) (\<lambda>n. if n = 2 then Some (Num r2) else <R (Suc 0) := s> (R n)))
+               (case_vname (\<lambda>n. if n = Suc 0 then Some (Num i) else input2state [] (Suc 0 + 1) (I n)) (\<lambda>n. if n = 2 then Some (Num r2) else <R (Suc 0) := s> (R n)))
                <R (Suc 0) := s', R 2 := Num r2>) = <R 1 := s, R 2 := Num (i+r2)>"
   apply (simp add: transitions)
   apply (rule ext)
