michael_formal/not4afp/Satisfaction.thy
@@ -1,0 +1,13 @@
+theory Satisfaction
+imports GExp
+begin
+
+lemma "\<not> satisfiable (gAnd (Gt (V (R 1)) (L (Num 100))) (Eq (V (R 1)) (L (Num 0))))"
+  apply (simp add: satisfiable_def)
+  apply clarify
+  apply (case_tac "MaybeBoolInt (\<lambda>x y. y < x) (s (R (Suc 0))) (Some (Num 100))")
+  by auto
+  
+
+
+end
